More general refinements in  ADTRefinement. Redid Cache Example. Still need to clean

ADTCache.v
@@ -3,140 +3,139 @@ Require Import Common Computation ADT Ensembles ADTRefinement.
 Generalizable All Variables.
 Set Implicit Arguments.
 
-  Open Scope comp_scope.
+Open Scope comp_scope.
 
-  Section addCache.
+Section addCache.
 
   (* A cache simply adds a new value to an ADT's representation [rep]. *)
 
-    Variable rep : Type.
-    Variable cacheTyp : Type.
+  Variable rep : Type.
+  Variable cacheTyp : Type.
 
-    Record cachedRep := cOb
-      { origRep : rep;
-        cachedVal : cacheTyp }.
+  Record cachedRep := cOb
+                        { origRep : rep;
+                          cachedVal : cacheTyp
+                        }.
 
-    (* There are two main ways of augmenting an ADT with a cache. *)
-
-    (* To add a cache, we update an ADT's mutators to include cached values.
+  (* To add a cache, we update an ADT's mutators to include cached values.
        We first running the old mutators
        to obtain the original mutated representation [or], then we add
        Pick implementation of the [cacheSpec] specification to the result. *)
 
-    Definition AddCacheEntry
-               {MutatorIndex}
-               (MutatorMethods : MutatorIndex -> mutatorMethodType rep)
-               (cacheSpec : rep -> nat -> cacheTyp -> Prop)
-               idx r n :=
-      or <- MutatorMethods idx (origRep r) n;
-      cv <- Pick (cacheSpec or n);
-      ret {| origRep := or;
-             cachedVal := cv |}.
+  Definition AddCacheEntry
+             {MutatorIndex}
+             (MutatorMethods : MutatorIndex -> mutatorMethodType rep)
+             (cacheSpec : rep -> cacheTyp -> Prop)
+             idx r n :=
+    or <- MutatorMethods idx (origRep r) n;
+    cv <- Pick (cacheSpec or);
+    ret {| origRep := or;
+           cachedVal := cv |}.
 
-    Variable repInv : Ensemble rep.
+  Variable repInv : Ensemble rep.
 
-    Definition ValidCacheInv 
-               (cacheSpec : rep -> nat -> cacheTyp -> Prop)
-               (n : nat) (r : cachedRep) :=
-      repInv (origRep r) /\ cacheSpec (origRep r) n (cachedVal r).
+  (* A representation augmented with a cache should satisfy the
+     original invariant [repInv], and the cache should satisfy [cacheSpec].*)
+  Definition ValidCacheInv
+             (cacheSpec : rep -> cacheTyp -> Prop)
+             (r : cachedRep) :=
+    repInv (origRep r) /\ cacheSpec (origRep r) (cachedVal r).
 
-    Lemma AddCacheEntryInv {MutatorIndex}:
-      forall
-        (MutatorMethods : MutatorIndex -> mutatorMethodType rep)
-        (MutatorMethodsInv :
-           forall (idx : MutatorIndex) (r : rep) (n : nat),
-             repInv r -> computational_inv repInv (MutatorMethods idx r n))
-        (cacheSpec : rep -> nat -> cacheTyp -> Prop)
-        (idx : MutatorIndex)
-        (r : cachedRep) (n : nat),
-        ValidCacheInv cacheSpec n r ->
-        computational_inv (ValidCacheInv cacheSpec n)
-                          (AddCacheEntry MutatorMethods cacheSpec idx r n).
-    Proof.
-      unfold AddCacheEntry, ValidCacheInv; simpl; intros.
-      inversion_by computes_to_inv; subst; eauto.
-    Qed.
-
-    End addCache.
-
-  Definition addCachedValue {cacheTyp} adt (cacheSpec : Rep adt -> nat -> cacheTyp -> Prop)
-  : ADT :=
-    {| Rep := cachedRep (Rep adt) cacheTyp;
-       RepInv r := exists n, ValidCacheInv (RepInv adt) cacheSpec n r;
-       ObserverIndex := ObserverIndex adt;
-       MutatorIndex := MutatorIndex adt;
-       ObserverMethods idx r := ObserverMethods adt idx (origRep r);
-       MutatorMethods idx r n :=
-         AddCacheEntry (MutatorMethods adt) cacheSpec idx r n;
-       MutatorMethodsInv := AddCacheEntryInv (MutatorMethodsInv adt) (cacheSpec := cacheSpec) |}.
-
-  Theorem refinesAddCachedValue
-          {cacheTyp}
-          adt
-          (cacheSpec : Rep adt -> cacheTyp -> Prop)
-  : refineADT adt (addCachedValue adt cacheSpec).
+  (* Mutators updated with [AddCacheEntry] preserve the [ValidCacheInv] invariant. *)
+  Lemma AddCacheEntryInv {MutatorIndex}:
+    forall
+      (MutatorMethods : MutatorIndex -> mutatorMethodType rep)
+      (MutatorMethodsInv :
+         forall (idx : MutatorIndex) (r : rep) (n : nat),
+           repInv r -> computational_inv repInv (MutatorMethods idx r n))
+      (cacheSpec : rep -> cacheTyp -> Prop),
+      mutatorInv
+        (fun r => ValidCacheInv cacheSpec r)
+        (AddCacheEntry MutatorMethods cacheSpec).
   Proof.
-    unfold addCachedValue, ValidCacheInv; destruct adt.
-    econstructor 1 with
-    (abs := fun r : cachedRep Rep cacheTyp =>  ret (origRep r))
-      (mutatorMap := @id MutatorIndex) (* Have to specify MutatorIndex in order to
-                                        unify- 8.5 might fix this? *)
-      (observerMap := @id ObserverIndex); simpl; unfold id; unfold AddCacheEntry;
-    intros; autorewrite with refine_monad.
-    - unfold refine; intros; inversion_by computes_to_inv; subst; eauto.
-    - reflexivity.
-    - inversion_by computes_to_inv; subst; eauto.
+    unfold AddCacheEntry, ValidCacheInv; simpl; intros.
+    inversion_by computes_to_inv; subst; eauto.
   Qed.
 
-  Definition replaceObserverCache adt
-             (ObserverIndex_eq : forall idx idx' : ObserverIndex adt, {idx = idx'} + {idx <> idx'})
-             (f : Rep adt -> nat -> Comp nat)
-             (cachedIndex : ObserverIndex adt)
-  : ADT :=
-    {| Rep := Rep adt;
-       RepInv := RepInv adt;
-       ObserverIndex := ObserverIndex adt;
-       MutatorIndex := MutatorIndex adt;
-       ObserverMethods idx :=
-         if (ObserverIndex_eq idx cachedIndex) then
-           f
-         else
-         ObserverMethods adt idx;
-       MutatorMethods := MutatorMethods adt;
-       MutatorMethodsInv := MutatorMethodsInv adt |}.
+End addCache.
 
-  Lemma refinesReplaceObserverCache
-             adt
-             (ObserverIndex_eq : forall idx idx' : ObserverIndex adt, {idx = idx'} + {idx <> idx'})
-             (f : Rep adt -> nat -> Comp nat)
-             (cachedIndex : ObserverIndex adt)
-             (refines_f : forall r n, RepInv adt r -> refine (ObserverMethods adt cachedIndex r n) (f r n))
-  : refineADT adt (replaceObserverCache adt ObserverIndex_eq f cachedIndex).
-  Proof.
-    unfold replaceObserverCache; destruct adt; simpl.
-    econstructor 1 with (abs := fun r : Rep => ret r)
-      (mutatorMap := @id MutatorIndex) (* Have to specify MutatorIndex in order to
-                                        unify- 8.5 might fix this? *)
-      (observerMap := @id ObserverIndex); simpl in *|-*; unfold id; intros;
-    autorewrite with refine_monad.
-    - reflexivity.
-    - find_if_inside; subst; [eauto | reflexivity].
-    - inversion_by computes_to_inv; subst; eauto.
-  Qed.
+Definition addCachedValue {cacheTyp} adt (cacheSpec : Rep adt -> cacheTyp -> Prop)
+: ADT :=
+  {| Rep := cachedRep (Rep adt) cacheTyp;
+     RepInv r := ValidCacheInv (RepInv adt) cacheSpec r; (* *)
+     ObserverIndex := ObserverIndex adt;
+     MutatorIndex := MutatorIndex adt;
+     ObserverMethods idx r := ObserverMethods adt idx (origRep r);
+     MutatorMethods := AddCacheEntry (MutatorMethods adt) cacheSpec;
+     MutatorMethodsInv := AddCacheEntryInv (MutatorMethodsInv adt) (cacheSpec := cacheSpec) |}.
 
-  Lemma refinesReplaceAddCache
+Theorem refinesAddCachedValue
+        {cacheTyp}
         adt
-        (ObserverIndex_eq : forall idx idx' : ObserverIndex adt, {idx = idx'} + {idx <> idx'})
-        (cacheSpec : Rep adt -> nat -> nat -> Prop)
-        (cachedIndex : ObserverIndex adt)
-        (refines_f : forall r n v, cacheSpec r n v ->
-                                   refine (ObserverMethods adt cachedIndex r n) (ret v))
-  : refineADT adt
-              (replaceObserverCache (addCachedValue adt cacheSpec)
-                                    ObserverIndex_eq (fun r _ => ret (cachedVal r)) cachedIndex).
-  Proof.
-    etransitivity. (* Example of where we can't rewrite? *)
-    eapply refinesAddCachedValue.
-    eapply refinesReplaceObserverCache.
-    unfold addCachedValue, ValidCacheInv; simpl; intuition.
-  Qed.
+        (cacheSpec : Rep adt -> cacheTyp -> Prop)
+: refineADT adt (addCachedValue adt cacheSpec).
+Proof.
+  unfold addCachedValue, ValidCacheInv; destruct adt.
+  econstructor 1 with
+  (abs := fun r : cachedRep Rep cacheTyp =>  ret (origRep r))
+    (mutatorMap := @id MutatorIndex) (* Have to specify MutatorIndex in order to
+                                        unify- 8.5 might fix this? *)
+    (observerMap := @id ObserverIndex); simpl; unfold id; unfold AddCacheEntry;
+  intros; autorewrite with refine_monad.
+  - unfold refine; intros; inversion_by computes_to_inv; subst; eauto.
+  - reflexivity.
+  - inversion_by computes_to_inv; subst; eauto.
+Qed.
+
+Definition replaceObserverCache adt
+           (ObserverIndex_eq : forall idx idx' : ObserverIndex adt, {idx = idx'} + {idx <> idx'})
+           (f : Rep adt -> nat -> Comp nat)
+           (cachedIndex : ObserverIndex adt)
+: ADT :=
+  {| Rep := Rep adt;
+     RepInv := RepInv adt;
+     ObserverIndex := ObserverIndex adt;
+     MutatorIndex := MutatorIndex adt;
+     ObserverMethods idx :=
+       if (ObserverIndex_eq idx cachedIndex) then
+         f
+       else
+         ObserverMethods adt idx;
+     MutatorMethods := MutatorMethods adt;
+     MutatorMethodsInv := MutatorMethodsInv adt |}.
+
+Lemma refinesReplaceObserverCache
+      adt
+      (ObserverIndex_eq : forall idx idx' : ObserverIndex adt, {idx = idx'} + {idx <> idx'})
+      (f : Rep adt -> nat -> Comp nat)
+      (cachedIndex : ObserverIndex adt)
+      (refines_f : forall r n, RepInv adt r -> refine (ObserverMethods adt cachedIndex r n) (f r n))
+: refineADT adt (replaceObserverCache adt ObserverIndex_eq f cachedIndex).
+Proof.
+  unfold replaceObserverCache; destruct adt; simpl.
+  econstructor 1 with (abs := fun r : Rep => ret r)
+                        (mutatorMap := @id MutatorIndex) (* Have to specify MutatorIndex in order to
+                                        unify- 8.5 might fix this? *)
+                        (observerMap := @id ObserverIndex); simpl in *|-*; unfold id; intros;
+                                                                    autorewrite with refine_monad.
+  - reflexivity.
+  - find_if_inside; subst; [eauto | reflexivity].
+  - inversion_by computes_to_inv; subst; eauto.
+Qed.
+
+Lemma refinesReplaceAddCache
+      adt
+      (ObserverIndex_eq : forall idx idx' : ObserverIndex adt, {idx = idx'} + {idx <> idx'})
+      (cacheSpec : Rep adt -> nat -> Prop)
+      (cachedIndex : ObserverIndex adt)
+      (refines_f : forall r n v, cacheSpec r v ->
+                                 refine (ObserverMethods adt cachedIndex r n) (ret v))
+: refineADT adt
+            (replaceObserverCache (addCachedValue adt cacheSpec)
+                                  ObserverIndex_eq (fun r _ => ret (cachedVal r)) cachedIndex).
+Proof.
+  etransitivity. (* Example of where we can't rewrite? *)
+  eapply refinesAddCachedValue.
+  eapply refinesReplaceObserverCache.
+  unfold addCachedValue, ValidCacheInv; simpl; intuition.
+Qed.
